src/Lean/Meta/Tactic/Grind/Arith/Cutsat/RelCnstr.lean
@@ -1,0 +1,77 @@
+/-
+Copyright (c) 2025 Amazon.com, Inc. or its affiliates. All Rights Reserved.
+Released under Apache 2.0 license as described in the file LICENSE.
+Authors: Leonardo de Moura
+-/
+prelude
+import Lean.Meta.Tactic.Simp.Arith.Int
+import Lean.Meta.Tactic.Grind.PropagatorAttr
+import Lean.Meta.Tactic.Grind.Arith.Cutsat.Var
+import Lean.Meta.Tactic.Grind.Arith.Cutsat.Proof
+
+namespace Lean.Meta.Grind.Arith.Cutsat
+def mkRelCnstrWithProof (c : RelCnstr) (h : RelCnstrProof) : GoalM RelCnstrWithProof := do
+  return { c, h, id := (← mkCnstrId) }
+
+abbrev RelCnstrWithProof.isUnsat (cₚ : RelCnstrWithProof) : Bool :=
+  cₚ.c.isUnsat
+
+abbrev RelCnstrWithProof.isTrivial (cₚ : RelCnstrWithProof) : Bool :=
+  cₚ.c.isTrivial
+
+abbrev RelCnstrWithProof.satisfied (cₚ : RelCnstrWithProof) : GoalM LBool :=
+  cₚ.c.satisfied
+
+def RelCnstrWithProof.norm (cₚ : RelCnstrWithProof) : GoalM RelCnstrWithProof := do
+  let cₚ ← if cₚ.c.isSorted then
+    pure cₚ
+  else
+    mkRelCnstrWithProof cₚ.c.norm (.norm cₚ)
+  let k := cₚ.c.gcdCoeffs
+  if k != 1 then
+    mkRelCnstrWithProof (cₚ.c.div k) (.divCoeffs cₚ)
+  else
+    return cₚ
+
+def assertRelCnstr (cₚ : RelCnstrWithProof) : GoalM Unit := do
+  if (← isInconsistent) then return ()
+  let cₚ ← cₚ.norm
+  if cₚ.isUnsat then
+    trace[grind.cutsat.le.unsat] "{← cₚ.denoteExpr}"
+    let hf ← withProofContext do
+      return mkApp4 (mkConst ``Int.Linear.RelCnstr.false_of_isUnsat_of_denote) (← getContext) (toExpr cₚ.c) reflBoolTrue (← cₚ.toExprProof)
+    closeGoal hf
+  else if cₚ.isTrivial then
+    trace[grind.cutsat.le.trivial] "{← cₚ.denoteExpr}"
+    return ()
+  else
+    -- TODO
+    return ()
+
+private def reportNonNormalized (e : Expr) : GoalM Unit := do
+  reportIssue! "unexpected non normalized inequality constraint found{indentExpr e}"
+
+private def toRelCnstr? (e : Expr) : GoalM (Option RelCnstr) := do
+  let_expr LE.le _ inst a b ← e | return none
+  unless (← isInstLEInt inst) do return none
+  let some k ← getIntValue? b
+    | reportNonNormalized e; return none
+  unless k == 0 do
+    reportNonNormalized e; return none
+  let p ← toPoly a
+  return some <| .le p
+
+/--
+Given an expression `e` that is in `True` (or `False` equivalence class), if `e` is an
+integer inequality, asserts it to the cutsat state.
+-/
+def propagateIfIntLe (e : Expr) (eqTrue : Bool) : GoalM Unit := do
+  let some c ← toRelCnstr? e | return ()
+  let cₚ ← if eqTrue then
+    mkRelCnstrWithProof c (.expr (← mkOfEqTrue (← mkEqTrueProof e)))
+  else
+    mkRelCnstrWithProof (c.mul (-1) |>.addConst 1) (.notExpr (← mkOfEqFalse (← mkEqFalseProof e)))
+  trace[grind.cutsat.assert.le] "{← cₚ.denoteExpr}"
+  assertRelCnstr cₚ
+
+end Lean.Meta.Grind.Arith.Cutsat
