src/Lean/Meta/Tactic/Grind/Arith/Cutsat/Util.lean
@@ -31,6 +31,17 @@ def DvdCnstr.isTrivial (c : DvdCnstr) : Bool :=
   | .num k' => k' % c.k == 0
   | _ => c.k == 1
 
+def RelCnstr.p : RelCnstr → Poly
+  | .eq p | .le p => p
+
+def RelCnstr.isSorted (c : RelCnstr) : Bool :=
+  c.p.isSorted
+
+def RelCnstr.isTrivial : RelCnstr → Bool
+  | .eq (.num 0) => true
+  | .le (.num k) => k ≤ 0
+  | _ => false
+
 end Int.Linear
 
 namespace Lean.Meta.Grind.Arith.Cutsat
@@ -61,6 +72,10 @@ def mkCnstrId : GoalM Nat := do
   return id
 
 def DvdCnstrWithProof.denoteExpr (cₚ : DvdCnstrWithProof) : GoalM Expr := do
+  let vars ← getVars
+  cₚ.c.denoteExpr (vars[·]!)
+
+def RelCnstrWithProof.denoteExpr (cₚ : RelCnstrWithProof) : GoalM Expr := do
   let vars ← getVars
   cₚ.c.denoteExpr (vars[·]!)
 
@@ -96,5 +111,38 @@ abbrev withProofContext (x : ProofM Expr) : GoalM Expr := do
   withLetDecl `ctx (mkApp (mkConst ``RArray) (mkConst ``Int)) (← toContextExpr) fun ctx => do
     let h ← x ctx |>.run' {}
     mkLetFVars #[ctx] h
+
+/--
+Tries to evaluate the polynomial `p` using the partial model/assignment built so far.
+The result is `none` if the polynomial contains variables that have not been assigned.
+-/
+def _root_.Int.Linear.Poly.eval? (p : Poly) : GoalM (Option Int) := do
+  let a := (← get').assignment
+  let rec go (v : Int) : Poly → Option Int
+    | .num k => some (v + k)
+    | .add k x p =>
+      if _ : x < a.size then
+        go (v + k*a[x]) p
+      else
+        none
+  return go 0 p
+
+/--
+Returns `.true` if `c` is satisfied by the current partial model,
+`.undef` if `c` contains unassigned variables, and `.false` otherwise.
+-/
+def _root_.Int.Linear.DvdCnstr.satisfied (c : DvdCnstr) : GoalM LBool := do
+  let some v ← c.p.eval? | return .undef
+  return decide (c.k ∣ v) |>.toLBool
+
+/--
+Returns `.true` if `c` is satisfied by the current partial model,
+`.undef` if `c` contains unassigned variables, and `.false` otherwise.
+-/
+def _root_.Int.Linear.RelCnstr.satisfied (c : RelCnstr) : GoalM LBool := do
+  let some v ← c.p.eval? | return .undef
+  match c with
+  | .eq _ => return v == 0 |>.toLBool
+  | .le _ => return decide (v <= 0) |>.toLBool
 
 end Lean.Meta.Grind.Arith.Cutsat
